safechecker/theories/PCUICConsistency.v
@@ -1,0 +1,220 @@
+(* The safe checker gives us a sound and complete wh-normalizer for
+   PCUIC, assuming strong normalization. Combined with canonicity,
+   this allows us to prove that PCUIC is consistent, i.e. there
+   is no axiom-free proof of [forall (P : Prop), P] in the empty
+   context. To do so we use weakening to add an empty inductive, the
+   provided term to build an inhabitant and then canonicity to show
+   that this is a contradiction. *)
+
+From Coq Require Import Ascii String.
+From Equations Require Import Equations.
+From MetaCoq.PCUIC Require Import PCUICAst.
+From MetaCoq.PCUIC Require Import PCUICAstUtils.
+From MetaCoq.PCUIC Require Import PCUICCanonicity.
+From MetaCoq.PCUIC Require Import PCUICInductiveInversion.
+From MetaCoq.PCUIC Require Import PCUICInversion.
+From MetaCoq.PCUIC Require Import PCUICLiftSubst.
+From MetaCoq.PCUIC Require Import PCUICSR.
+From MetaCoq.PCUIC Require Import PCUICSafeLemmata.
+From MetaCoq.PCUIC Require Import PCUICTyping.
+From MetaCoq.PCUIC Require Import PCUICUnivSubst.
+From MetaCoq.PCUIC Require Import PCUICValidity.
+From MetaCoq.PCUIC Require Import PCUICWeakeningEnv.
+From MetaCoq.Template Require Import config utils.
+From MetaCoq.SafeChecker Require Import PCUICSafeReduce.
+
+Local Opaque hnf.
+
+Fixpoint string_repeat c (n : nat) : string :=
+  match n with
+  | 0 => ""
+  | S n => String c (string_repeat c n)
+  end.
+
+Lemma string_repeat_length c n :
+  String.length (string_repeat c n) = n.
+Proof.
+  induction n; cbn; auto.
+Qed.
+
+Definition max_name_length (Σ : global_env) : nat :=
+  fold_right max 0 (map (fun '(kn, _) => String.length (string_of_kername kn)) Σ).
+
+Lemma max_name_length_ge Σ :
+  Forall (fun '(kn, _) => String.length (string_of_kername kn) <= max_name_length Σ) Σ.
+Proof.
+  induction Σ as [|(kn&decl) Σ IH]; cbn; constructor.
+  - lia.
+  - eapply Forall_impl; eauto.
+    intros (?&?); cbn; intros.
+    fold (max_name_length Σ).
+    lia.
+Qed.
+
+Definition make_fresh_name (Σ : global_env) : kername :=
+  (MPfile [], string_repeat "a"%char (S (max_name_length Σ))).
+
+Lemma make_fresh_name_fresh Σ :
+  fresh_global (make_fresh_name Σ) Σ.
+Proof.
+  pose proof (max_name_length_ge Σ) as all.
+  eapply Forall_impl; eauto.
+  cbn.
+  intros (kn&decl) le.
+  cbn.
+  intros ->.
+  unfold make_fresh_name in le.
+  cbn in le.
+  rewrite string_repeat_length in le.
+  lia.
+Qed.
+
+Definition Prop_univ := Universe.of_levels (inl PropLevel.lProp).
+
+Definition False_oib : one_inductive_body :=
+  {| ind_name := "";
+     ind_type := tSort Prop_univ;
+     ind_kelim := IntoAny;
+     ind_ctors := [];
+     ind_projs := [];
+     ind_relevance := Relevant |}.
+
+Definition False_mib : mutual_inductive_body :=
+  {| ind_finite := BiFinite;
+     ind_npars := 0;
+     ind_params := [];
+     ind_bodies := [False_oib];
+     ind_universes := Monomorphic_ctx ContextSet.empty;
+     ind_variance := None |}.
+
+Definition axiom_free Σ :=
+  forall c decl, declared_constant Σ c decl -> cst_body decl <> None.
+
+Lemma axiom_free_axiom_free_value Σ t :
+  axiom_free Σ ->
+  axiom_free_value Σ [] t.
+Proof.
+  intros axfree.
+  cut (Forall is_true []); [|constructor].
+  generalize ([] : list bool).
+  induction t; intros axfree_args all_true; cbn; auto.
+  - destruct lookup_env eqn:find; auto.
+    destruct g; auto.
+    destruct c; auto.
+    apply axfree in find; cbn in *.
+    now destruct cst_body.
+  - destruct nth_error; auto.
+    rewrite nth_nth_error.
+    destruct nth_error eqn:nth; auto.
+    eapply nth_error_forall in nth; eauto.
+Qed.
+
+Definition binder := {| binder_name := nNamed "P"; binder_relevance := Relevant |}.
+
+Theorem pcuic_consistent {cf:checker_flags} Σ t :
+  wf_ext Σ ->
+  axiom_free Σ ->
+  (* t : forall (P : Prop), P *)
+  Σ ;;; [] |- t : tProd binder (tSort Prop_univ) (tRel 0) ->
+  False.
+Proof.
+  intros wfΣ axfree cons.
+  set (Σext := ((make_fresh_name Σ, InductiveDecl False_mib) :: Σ.1, Σ.2)).
+  assert (wf': wf_ext Σext).
+  { constructor; [constructor|].
+    - destruct wfΣ; auto.
+    - apply make_fresh_name_fresh.
+    - red.
+      cbn.
+      split.
+      { now intros ? ?%LevelSet.empty_spec. }
+      split.
+      { now intros ? ?%ConstraintSet.empty_spec. }
+      split; auto.
+      destruct wfΣ as (?&(?&?&?&[val sat])).
+      exists val.
+      intros l isin.
+      apply sat; auto.
+      apply ConstraintSet.union_spec.
+      apply ConstraintSet.union_spec in isin as [?%ConstraintSet.empty_spec|]; auto.
+    - hnf.
+      constructor.
+      + constructor.
+        * econstructor; cbn.
+          -- instantiate (2 := []); reflexivity.
+          -- exists (Universe.super Prop_univ).
+             constructor; auto.
+             constructor.
+          -- instantiate (1 := []).
+             constructor.
+          --  intros.
+              congruence.
+          -- constructor.
+          -- intros ? [=].
+        * constructor.
+      + constructor.
+      + reflexivity.
+      + reflexivity.
+    - destruct wfΣ; auto. }
+  eapply (env_prop_typing _ _ PCUICWeakeningEnv.weakening_env) in cons; auto.
+  3: exists [(make_fresh_name Σ, InductiveDecl False_mib)]; reflexivity.
+  2: now destruct wf'.
+  
+  set (Σ' := _ ++ _) in cons.
+  set (False_ty := tInd (mkInd (make_fresh_name Σ) 0) []).
+  assert (typ_false: (Σ', Σ.2);;; [] |- tApp t False_ty : False_ty).
+  { apply validity_term in cons as typ_prod; auto.
+    destruct typ_prod.
+    eapply type_App with (B := tRel 0) (u := False_ty); eauto.
+    eapply type_Ind with (u := []) (mdecl := False_mib) (idecl := False_oib); eauto.
+    - hnf.
+      cbn.
+      unfold declared_minductive.
+      cbn.
+      rewrite eq_kername_refl.
+      auto.
+    - cbn.
+      auto. }
+  assert (sqwf: ∥ wf (Σ', Σ.2).1 ∥) by now destruct wf'.
+  pose proof (iswelltyped _ _ _ _ typ_false) as wt.
+  pose proof (@hnf_sound _ _ sqwf _ _ wt) as [r].
+  pose proof (@hnf_complete _ _ sqwf _ _ wt) as [w].
+  eapply subject_reduction in typ_false; eauto.
+  eapply whnf_ind_finite with (indargs := []) in typ_false as ctor; auto.
+  - unfold isConstruct_app in ctor.
+    destruct decompose_app eqn:decomp.
+    apply decompose_app_inv in decomp.
+    rewrite decomp in typ_false.
+    destruct t0; try discriminate ctor.
+    apply inversion_mkApps in typ_false as H; auto.
+    destruct H as (?&typ_ctor&_).
+    apply inversion_Construct in typ_ctor as (?&?&?&?&?&?&?); auto.
+    unshelve eapply Construct_Ind_ind_eq with (args' := []) in typ_false.
+    5: eassumption.
+    1: eauto.
+    destruct on_declared_constructor.
+    destruct p.
+    destruct s.
+    destruct p.
+    destruct typ_false as ((((->&_)&_)&_)&_).
+    clear -d.
+    destruct d as ((?&?)&?).
+    cbn in *.
+    red in H.
+    cbn in *.
+    rewrite eq_kername_refl in H.
+    noconf H.
+    noconf H0.
+    cbn in H1.
+    rewrite nth_error_nil in H1.
+    discriminate.
+  - eapply axiom_free_axiom_free_value.
+    intros kn decl isdecl.
+    hnf in isdecl.
+    cbn in isdecl.
+    destruct eq_kername; [noconf isdecl|].
+    eapply axfree; eauto.
+  - unfold check_recursivity_kind.
+    cbn.
+    rewrite eq_kername_refl; auto.
+Qed.
